Adding alternative list based case

theories/Semantics/Cbn.v
@@ -1,78 +1,27 @@
-From Stdlib Require Import List Utf8 Relations Relation_Operators Vectors.Fin Program.Equality.
+From Stdlib Require Import List Utf8 Relations Relation_Operators.
 
 From Cyclic.Syntax Require Import StrictPos Term.
 
 Import ListNotations.
-Import StrictPos.
 Import Term.Syntax.
 
 Set Default Proof Using "Type".
 
 (* Call-by-name (weak-head) operational semantics for raw terms.
 
-   This is a small-step semantics that only reduces in:
-   - the function position of an application
-   - the scrutinee position of a case
-   - the top-level of a fix
+   We reduce only in:
+   - function position of application
+   - scrutinee position of case
+   - the head of a fix
 
    Arguments are never evaluated before substitution.
 *)
-
-Fixpoint enumFin (n : nat) : list (Fin.t n) :=
-  match n with
-  | 0 => []
-  | S n' => Fin.F1 :: map Fin.FS (enumFin n')
-  end.
 
 Fixpoint apps (t : tm) (us : list tm) : tm :=
   match us with
   | [] => t
   | u :: us => apps (tApp t u) us
   end.
-
-Definition roll_params (Σ : ind_sig ty) (s : Shape Σ) (params : ParamPos Σ s -> tm) : list tm :=
-  map params (enumFin (param_arity Σ s)).
-
-Definition roll_args (Σ : ind_sig ty) (s : Shape Σ) (k : Pos Σ s -> tm) : list tm :=
-  map k (enumFin (arity Σ s)).
-
-Fixpoint shift (d : nat) (c : nat) (t : tm) : tm :=
-  match t with
-  | tVar x => if Nat.ltb x c then tVar x else tVar (x + d)
-  | tLam A t => tLam A (shift d (S c) t)
-  | tApp t u => tApp (shift d c t) (shift d c u)
-  | tFix A t => tFix A (shift d (S c) t)
-  | tRoll Σ s params k =>
-      tRoll Σ s
-        (fun i => shift d c (params i))
-        (fun j => shift d c (k j))
-  | tCase Σ scrut C br =>
-      tCase Σ (shift d c scrut) C (fun s => shift d c (br s))
-  end.
-
-Definition up (σ : nat -> tm) : nat -> tm :=
-  fun x =>
-    match x with
-    | 0 => tVar 0
-    | S x => shift 1 0 (σ x)
-    end.
-
-Fixpoint subst (σ : nat -> tm) (t : tm) : tm :=
-  match t with
-  | tVar x => σ x
-  | tLam A t => tLam A (subst (up σ) t)
-  | tApp t u => tApp (subst σ t) (subst σ u)
-  | tFix A t => tFix A (subst (up σ) t)
-  | tRoll Σ s params k =>
-      tRoll Σ s
-        (fun i => subst σ (params i))
-        (fun j => subst σ (k j))
-  | tCase Σ scrut C br =>
-      tCase Σ (subst σ scrut) C (fun s => subst σ (br s))
-  end.
-
-Definition subst0 (u : tm) (t : tm) : tm :=
-  subst (fun x => match x with 0 => u | S x => tVar x end) t.
 
 Inductive step : tm -> tm -> Prop :=
 | step_beta A t u :
@@ -82,32 +31,32 @@ Inductive step : tm -> tm -> Prop :=
     step (tApp t u) (tApp t' u)
 | step_fix A t :
     step (tFix A t) (subst0 (tFix A t) t)
-| step_case_scrut Σ scrut scrut' C br :
+| step_case_scrut I scrut scrut' C brs :
     step scrut scrut' ->
-    step (tCase Σ scrut C br) (tCase Σ scrut' C br)
-| step_case_roll Σ s params k C br :
-    step (tCase Σ (tRoll Σ s params k) C br)
-      (apps (br s) (roll_params Σ s params ++ roll_args Σ s k)).
+    step (tCase I scrut C brs) (tCase I scrut' C brs)
+| step_case_roll I c params recs C brs br :
+    branch brs c = Some br ->
+    step (tCase I (tRoll I c params recs) C brs)
+      (apps br (params ++ recs)).
 
 Definition steps : tm -> tm -> Prop :=
   clos_refl_trans tm step.
 
 Inductive value : tm -> Prop :=
 | v_lam A t : value (tLam A t)
-| v_roll Σ s params k : value (tRoll Σ s params k).
+| v_roll I c params recs : value (tRoll I c params recs).
 
 (* Neutrals are stuck at the head (no CBN reduction possible). *)
 Inductive neutral : tm -> Prop :=
 | ne_var x : neutral (tVar x)
 | ne_app t u : neutral t -> neutral (tApp t u)
-| ne_case Σ t C br : neutral t -> neutral (tCase Σ t C br).
+| ne_case I t C brs : neutral t -> neutral (tCase I t C brs).
 
 (* Weak-head normal forms: values or neutrals. *)
 Inductive whnf : tm -> Prop :=
 | whnf_val v : value v -> whnf v
 | whnf_ne t : neutral t -> whnf t.
 
-(* Explicit weak-head evaluation: reduce to a WHNF. *)
 Definition eval_whnf (t w : tm) : Prop :=
   steps t w ∧ whnf w.
 
@@ -121,192 +70,3 @@ Definition terminates (t : tm) : Prop :=
 
 CoInductive diverges (t : tm) : Prop :=
 | diverges_step t' : step t t' -> diverges t' -> diverges t.
-
-Lemma value_no_step (v v' : tm) :
-  value v -> step v v' -> False.
-Proof.
-  intros Hv Hstep.
-  inversion Hv; subst; inversion Hstep.
-Qed.
-
-Lemma neutral_no_step (t t' : tm) :
-  neutral t -> step t t' -> False.
-Proof.
-  intro Hn.
-  revert t'.
-  induction Hn as [x|t u Ht IH|Σ t C br Ht IH]; intro t'; intro Hstep.
-  - inversion Hstep.
-  - inversion Hstep; subst.
-    + inversion Ht.
-    + eapply IH; eauto.
-  - inversion Hstep; subst.
-    + eapply IH; eauto.
-    + inversion Ht.
-Qed.
-
-Lemma whnf_no_step (t t' : tm) :
-  whnf t -> step t t' -> False.
-Proof.
-  intros Hwh Hstep.
-  inversion Hwh; subst.
-  - exact (value_no_step _ _ H Hstep).
-  - exact (neutral_no_step _ _ H Hstep).
-Qed.
-
-(* Determinism of call-by-name stepping. *)
-Lemma step_deterministic (t t1 t2 : tm) :
-  step t t1 -> step t t2 -> t1 = t2.
-Proof.
-  intro H1.
-  revert t2.
-  induction H1 as
-    [A t u
-    | t t' u Htt' IH
-    | A t
-    | Σ scrut scrut' C br Hscrut IH
-    | Σ s params k C br];
-    intro t2; intro H2.
-  - inversion H2; subst; try reflexivity; try discriminate.
-    exfalso.
-    match goal with
-    | H : step (tLam _ _) _ |- _ => eapply value_no_step; [apply v_lam|exact H]
-    end.
-  - inversion H2; subst; try discriminate.
-    { exfalso.
-      match goal with
-      | H : step (tLam _ _) _ |- _ => eapply value_no_step; [apply v_lam|exact H]
-      end. }
-    { f_equal. eapply IH; eauto. }
-  - inversion H2; subst; reflexivity.
-  - inversion H2; subst; try discriminate.
-    { (* case-scrut vs case-scrut *)
-      repeat match goal with
-      | H : existT _ _ _ = existT _ _ _ |- _ => dependent destruction H
-      end.
-      match goal with
-      | H : step scrut ?u |- _ => pose proof (IH _ H) as ->
-      end.
-      reflexivity. }
-    { (* case-scrut vs case-roll is impossible: scrut is a roll, but rolls don't step *)
-      exfalso.
-      eapply value_no_step.
-      - apply v_roll.
-      - exact Hscrut. }
-  - inversion H2; subst; try discriminate.
-    { (* case-roll vs case-scrut is impossible: rolls don't step *)
-      exfalso.
-      match goal with
-      | H : step (tRoll _ _ _ _) _ |- _ => eapply value_no_step; [apply v_roll|exact H]
-      end. }
-    { (* case-roll vs case-roll *)
-      repeat match goal with
-      | H : existT _ _ _ = existT _ _ _ |- _ => dependent destruction H
-      end.
-      reflexivity. }
-Qed.
-
-(* A helper for reasoning about multi-step reductions. *)
-Lemma steps_eq_or_step (t u : tm) :
-  steps t u -> t = u ∨ ∃ t', step t t' ∧ steps t' u.
-Proof.
-  intro H.
-  induction H.
-  - (* rt_step *)
-    right. exists y. split; [exact H|apply rt_refl].
-  - (* rt_refl *)
-    left. reflexivity.
-  - (* rt_trans *)
-    destruct IHclos_refl_trans1 as [->|[t' [Ht' Ht'y]]].
-    + exact IHclos_refl_trans2.
-    + right. exists t'. split.
-      * exact Ht'.
-      * eapply rt_trans; eauto.
-Qed.
-
-Lemma whnf_stuck (w u : tm) :
-  whnf w -> steps w u -> u = w.
-Proof.
-  intros Hwh Hwu.
-  destruct (steps_eq_or_step _ _ Hwu) as [->|[w' [Hwstep _]]].
-  - reflexivity.
-  - exfalso. exact (whnf_no_step _ _ Hwh Hwstep).
-Qed.
-
-Lemma steps_compare (t u v : tm) :
-  steps t u -> steps t v -> steps u v ∨ steps v u.
-Proof.
-  intro Htu.
-  revert v.
-  induction Htu; intro v; intro Htv.
-  - (* rt_step *)
-    destruct (steps_eq_or_step _ _ Htv) as [Heq|[t' [Ht' Ht'v]]].
-    + subst. right. apply rt_step. exact H.
-    + assert (t' = y) by (eapply step_deterministic; eauto).
-      subst t'. left. exact Ht'v.
-  - (* rt_refl *)
-    left. exact Htv.
-  - (* rt_trans *)
-    specialize (IHHtu1 _ Htv) as [Hyv|Hvy].
-    + exact (IHHtu2 _ Hyv).
-    + right. eapply rt_trans; eauto.
-Qed.
-
-Theorem eval_whnf_deterministic (t w1 w2 : tm) :
-  t ⇓wh w1 -> t ⇓wh w2 -> w1 = w2.
-Proof.
-  intros [Ht1 Hw1] [Ht2 Hw2].
-  destruct (steps_compare _ _ _ Ht1 Ht2) as [H12|H21].
-  - symmetry. exact (whnf_stuck _ _ Hw1 H12).
-  - exact (whnf_stuck _ _ Hw2 H21).
-Qed.
-
-(* Big-step weak-head evaluation (inductive), equivalent to ⇓wh. *)
-Inductive eval_whnf_big : tm -> tm -> Prop :=
-| ewhnf_done w : whnf w -> eval_whnf_big w w
-| ewhnf_step t t' w : step t t' -> eval_whnf_big t' w -> eval_whnf_big t w.
-
-Lemma eval_whnf_big_sound (t w : tm) :
-  eval_whnf_big t w -> t ⇓wh w.
-Proof.
-  intro He.
-  induction He as [w Hwh|t t' w Hstep He IH].
-  - split.
-    + apply rt_refl.
-    + exact Hwh.
-  - destruct IH as [Ht'w Hwh].
-    split.
-    + eapply rt_trans.
-      * apply rt_step. exact Hstep.
-      * exact Ht'w.
-    + exact Hwh.
-Qed.
-
-Lemma eval_whnf_big_of_steps (t0 u w : tm) :
-  steps t0 u -> eval_whnf_big u w -> eval_whnf_big t0 w.
-Proof.
-  intro Htu.
-  revert w.
-  dependent induction Htu; intros w He.
-  - (* rt_step *) exact (ewhnf_step _ _ _ H He).
-  - (* rt_refl *) exact He.
-  - (* rt_trans *)
-    apply IHHtu1.
-    apply IHHtu2.
-    exact He.
-Qed.
-
-Lemma eval_whnf_big_complete (t w : tm) :
-  t ⇓wh w -> eval_whnf_big t w.
-Proof.
-  intros [Htw Hwh].
-  apply (eval_whnf_big_of_steps t w w Htw).
-  exact (ewhnf_done w Hwh).
-Qed.
-
-Theorem eval_whnf_big_deterministic (t w1 w2 : tm) :
-  eval_whnf_big t w1 -> eval_whnf_big t w2 -> w1 = w2.
-Proof.
-  intros H1 H2.
-  apply (eval_whnf_deterministic t w1 w2);
-    apply eval_whnf_big_sound; assumption.
-Qed.
