theories/Syntax/Term.v
@@ -1,5 +1,6 @@
-From Stdlib Require Import List Arith Lia Utf8 FunctionalExtensionality Wellfounded Program.Equality.
-From Stdlib.Vectors Require Import Fin Vector VectorSpec.
+From Stdlib Require Import List Arith Utf8.
+
+From Autosubst Require Import Autosubst.
 
 From Cyclic.Syntax Require Import StrictPos.
 
@@ -9,361 +10,42 @@ Set Default Proof Using "Type".
 
 Module Syntax.
   Inductive tm : Type :=
-  | tVar (x : nat)
+  | tVar (x : var)
   | tSort (i : nat)
-  | tPi (A : tm) (B : tm)
-  | tLam (A : tm) (t : tm)
+  | tPi (A : tm) (B : {bind tm})
+  | tLam (A : tm) (t : {bind tm})
   | tApp (t u : tm)
-  | tFix (A : tm) (t : tm)
+  | tFix (A : tm) (t : {bind tm})
   | tInd (I : nat)
   | tRoll (I : nat) (c : nat) (params recs : list tm)
-  | tCase (I : nat) (n : nat) (scrut : tm) (C : tm) (brs : Vector.t tm n).
+  | tCase (I : nat) (scrut : tm) (C : tm) (brs : list tm).
 
-  Definition branch {n} (brs : Vector.t tm n) (k : Fin.t n) : tm :=
-    Vector.nth brs k.
+  Definition branch (brs : list tm) (c : nat) : option tm :=
+    nth_error brs c.
 
-  Fixpoint shift (d : nat) (c : nat) (t : tm) : tm :=
-    match t with
-    | tVar x => if Nat.ltb x c then tVar x else tVar (x + d)
-    | tSort i => tSort i
-    | tPi A B => tPi (shift d c A) (shift d (S c) B)
-    | tLam A t => tLam (shift d c A) (shift d (S c) t)
-    | tApp t u => tApp (shift d c t) (shift d c u)
-    | tFix A t => tFix (shift d c A) (shift d (S c) t)
-    | tInd ind => tInd ind
-    | tRoll ind ctor ps rs =>
-        tRoll ind ctor (List.map (shift d c) ps) (List.map (shift d c) rs)
-    | tCase ind n scrut C brs =>
-        tCase ind n (shift d c scrut) (shift d c C) (Vector.map (shift d c) brs)
-    end.
+  Global Instance Ids_tm : Ids tm := tVar.
+  Global Instance Rename_tm : Rename tm. derive. Defined.
+  Global Instance Subst_tm : Subst tm. derive. Defined.
+  Global Instance SubstLemmas_tm : SubstLemmas tm. derive. Qed.
 
-  Definition up (σ : nat -> tm) : nat -> tm :=
-    fun x => match x with 0 => tVar 0 | S x => shift 1 0 (σ x) end.
+  Definition ids : var -> tm :=
+    @Autosubst_Classes.ids tm Ids_tm.
 
-  Fixpoint subst (σ : nat -> tm) (t : tm) : tm :=
-    match t with
-    | tVar x => σ x
-    | tSort i => tSort i
-    | tPi A B => tPi (subst σ A) (subst (up σ) B)
-    | tLam A t => tLam (subst σ A) (subst (up σ) t)
-    | tApp t u => tApp (subst σ t) (subst σ u)
-    | tFix A t => tFix (subst σ A) (subst (up σ) t)
-    | tInd ind => tInd ind
-    | tRoll ind ctor ps rs =>
-        tRoll ind ctor (List.map (subst σ) ps) (List.map (subst σ) rs)
-    | tCase ind n scrut C brs =>
-        tCase ind n (subst σ scrut) (subst σ C) (Vector.map (subst σ) brs)
-    end.
+  Definition rename : (var -> var) -> tm -> tm :=
+    @Autosubst_Classes.rename tm Rename_tm.
+
+  Definition subst : (var -> tm) -> tm -> tm :=
+    @Autosubst_Classes.subst tm Subst_tm.
+
+  Definition up : (var -> tm) -> var -> tm :=
+    @Autosubst_Classes.up tm Ids_tm Rename_tm.
 
   Definition subst0 (u : tm) (t : tm) : tm :=
-    subst (fun x => match x with 0 => u | S x => tVar x end) t.
+    t.[u/].
 
-  Module Lemmas.
-    Fixpoint sum_list (ns : list nat) : nat :=
-      match ns with
-      | [] => 0
-      | n :: ns => n + sum_list ns
-      end.
+  Definition shift_sub (d c : nat) : var -> var :=
+    fun x => if x <? c then x else x + d.
 
-    Fixpoint sum_fin (n : nat) (f : Fin.t n -> nat) : nat :=
-      match n as n0 return (Fin.t n0 -> nat) -> nat with
-      | 0 => fun _ => 0
-      | S n => fun f => f Fin.F1 + sum_fin n (fun k => f (Fin.FS k))
-      end f.
-
-    Fixpoint size (t : tm) : nat :=
-      match t with
-      | tVar _ => 1
-      | tSort _ => 1
-      | tPi A B => 1 + size A + size B
-      | tLam A t => 1 + size A + size t
-      | tApp t u => 1 + size t + size u
-      | tFix A t => 1 + size A + size t
-      | tInd _ => 1
-      | tRoll _ _ ps rs => 1 + sum_list (List.map size ps) + sum_list (List.map size rs)
-      | tCase _ n scrut C brs =>
-          1 + size scrut + size C + sum_fin n (fun k => size (branch brs k))
-      end.
-
-    Definition wf_tm : well_founded (fun t1 t2 => size t1 < size t2) :=
-      wf_inverse_image _ _ lt size Nat.lt_wf_0.
-
-    Lemma size_le_sum_list {ps : list tm} {p : tm} :
-      List.In p ps -> size p <= sum_list (List.map size ps).
-    Proof.
-      intro Hin.
-      induction ps as [|q qs IH]; simpl in *.
-      - contradiction.
-      - destruct Hin as [Hin|Hin]; subst.
-        + lia.
-        + specialize (IH Hin).
-          lia.
-    Qed.
-
-    Lemma size_lt_roll_param {I c} {params recs : list tm} {p : tm} :
-      List.In p params -> size p < size (tRoll I c params recs).
-    Proof.
-      intro Hin.
-      simpl.
-      pose proof (size_le_sum_list (ps:=params) (p:=p) Hin) as Hle.
-      lia.
-    Qed.
-
-    Lemma size_lt_roll_rec {I c} {params recs : list tm} {r : tm} :
-      List.In r recs -> size r < size (tRoll I c params recs).
-    Proof.
-      intro Hin.
-      simpl.
-      pose proof (size_le_sum_list (ps:=recs) (p:=r) Hin) as Hle.
-      lia.
-    Qed.
-
-    Lemma size_le_sum_fin {n} (brs : Vector.t tm n) (k : Fin.t n) :
-      size (branch brs k) <= sum_fin n (fun j => size (branch brs j)).
-    Proof.
-      revert brs k.
-      induction n as [|n IH]; intros brs k.
-      - inversion k.
-      - dependent destruction brs.
-        dependent destruction k.
-        + simpl. lia.
-        + simpl.
-          specialize (IH brs k).
-          lia.
-    Qed.
-
-    Lemma size_lt_case_branch {I n} {scrut C : tm} {brs : Vector.t tm n} (k : Fin.t n) :
-      size (branch brs k) < size (tCase I n scrut C brs).
-    Proof.
-      simpl.
-      pose proof (size_le_sum_fin brs k) as Hle.
-      lia.
-    Qed.
-
-    Definition shift_sub (d c : nat) : nat -> tm :=
-      fun x => if Nat.ltb x c then tVar x else tVar (x + d).
-
-    Lemma up_shift_sub d c : up (shift_sub d c) = shift_sub d (S c).
-    Proof.
-      apply functional_extensionality; intro x.
-      destruct x as [|x]; simpl.
-      - reflexivity.
-      - unfold shift_sub.
-        destruct (Nat.ltb x c) eqn:Hlt.
-        + apply Nat.ltb_lt in Hlt.
-          assert (Nat.ltb (S x) (S c) = true) as Hlt'.
-          { apply Nat.ltb_lt. lia. }
-          rewrite Hlt'.
-          simpl.
-          f_equal.
-          lia.
-        + apply Nat.ltb_ge in Hlt.
-          assert (Nat.ltb (S x) (S c) = false) as Hge'.
-          { apply Nat.ltb_ge. lia. }
-          rewrite Hge'.
-          simpl.
-          f_equal.
-          lia.
-    Qed.
-
-    Lemma up_ext (σ τ : nat -> tm) :
-      (forall x, σ x = τ x) -> forall x, up σ x = up τ x.
-    Proof.
-      intro Heq.
-      intro x.
-      destruct x as [|x]; simpl; [reflexivity|].
-      rewrite Heq.
-      reflexivity.
-    Qed.
-
-    Lemma subst_ext (σ τ : nat -> tm) (t : tm) :
-      (forall x, σ x = τ x) -> subst σ t = subst τ t.
-    Proof.
-      intro Heq.
-      revert σ τ Heq.
-      refine (well_founded_induction wf_tm
-        (fun t => forall σ τ, (forall x, σ x = τ x) -> subst σ t = subst τ t)
-        _ t).
-      intros t0 IH σ τ Heq0.
-      destruct t0 as
-        [x|i|A B|A body|fn arg|A body|ind|ind ctor params recs|ind n scrut C brs];
-        simpl; try reflexivity.
-      - exact (Heq0 x).
-      - f_equal.
-        + assert (Hlt : size A < size (tPi A B)) by (simpl; lia).
-          exact (IH A Hlt σ τ Heq0).
-        + assert (Hlt : size B < size (tPi A B)) by (simpl; lia).
-          exact (IH B Hlt (up σ) (up τ) (up_ext _ _ Heq0)).
-      - f_equal.
-        + assert (Hlt : size A < size (tLam A body)) by (simpl; lia).
-          exact (IH A Hlt σ τ Heq0).
-        + assert (Hlt : size body < size (tLam A body)) by (simpl; lia).
-          exact (IH body Hlt (up σ) (up τ) (up_ext _ _ Heq0)).
-      - f_equal.
-        + assert (Hlt : size fn < size (tApp fn arg)) by (simpl; lia).
-          exact (IH fn Hlt σ τ Heq0).
-        + assert (Hlt : size arg < size (tApp fn arg)) by (simpl; lia).
-          exact (IH arg Hlt σ τ Heq0).
-      - f_equal.
-        + assert (Hlt : size A < size (tFix A body)) by (simpl; lia).
-          exact (IH A Hlt σ τ Heq0).
-        + assert (Hlt : size body < size (tFix A body)) by (simpl; lia).
-          exact (IH body Hlt (up σ) (up τ) (up_ext _ _ Heq0)).
-      - f_equal.
-        + apply List.map_ext_in.
-          intros p Hp.
-          pose proof (size_lt_roll_param (I:=ind) (c:=ctor) (params:=params) (recs:=recs) (p:=p) Hp) as Hlt.
-          exact (IH p Hlt σ τ Heq0).
-        + apply List.map_ext_in.
-          intros r Hr.
-          pose proof (size_lt_roll_rec (I:=ind) (c:=ctor) (params:=params) (recs:=recs) (r:=r) Hr) as Hlt.
-          exact (IH r Hlt σ τ Heq0).
-      - f_equal.
-        + assert (Hlt : size scrut < size (tCase ind n scrut C brs)) by (simpl; lia).
-          exact (IH scrut Hlt σ τ Heq0).
-        + assert (Hlt : size C < size (tCase ind n scrut C brs)) by (simpl; lia).
-          exact (IH C Hlt σ τ Heq0).
-        + apply (proj1 (VectorSpec.eq_nth_iff _ _
-            (Vector.map (subst σ) brs)
-            (Vector.map (subst τ) brs))).
-          intros p1 p2 Hp.
-          subst p2.
-          rewrite (VectorSpec.nth_map (subst σ) brs p1 p1 eq_refl).
-          rewrite (VectorSpec.nth_map (subst τ) brs p1 p1 eq_refl).
-          pose proof (size_lt_case_branch (I:=ind) (n:=n) (scrut:=scrut) (C:=C) (brs:=brs) p1) as Hlt.
-          exact (IH (branch brs p1) Hlt σ τ Heq0).
-    Qed.
-
-    Lemma shift_as_subst (d c : nat) (t : tm) :
-      shift d c t = subst (shift_sub d c) t.
-    Proof.
-      revert c.
-      refine (well_founded_induction wf_tm
-        (fun t => forall c, shift d c t = subst (shift_sub d c) t)
-        _ t).
-      intros t0 IH c0.
-      destruct t0 as
-        [x|i|A B|A body|fn arg|A body|ind|ind ctor params recs|ind n scrut C brs];
-        simpl; try reflexivity.
-      - apply f_equal2.
-        + assert (Hlt : size A < size (tPi A B)) by (simpl; lia).
-          exact (IH A Hlt c0).
-        + rewrite up_shift_sub.
-          assert (Hlt : size B < size (tPi A B)) by (simpl; lia).
-          exact (IH B Hlt (S c0)).
-      - apply f_equal2.
-        + assert (Hlt : size A < size (tLam A body)) by (simpl; lia).
-          exact (IH A Hlt c0).
-        + rewrite up_shift_sub.
-          assert (Hlt : size body < size (tLam A body)) by (simpl; lia).
-          exact (IH body Hlt (S c0)).
-      - apply f_equal2.
-        + assert (Hlt : size fn < size (tApp fn arg)) by (simpl; lia).
-          exact (IH fn Hlt c0).
-        + assert (Hlt : size arg < size (tApp fn arg)) by (simpl; lia).
-          exact (IH arg Hlt c0).
-      - apply f_equal2.
-        + assert (Hlt : size A < size (tFix A body)) by (simpl; lia).
-          exact (IH A Hlt c0).
-        + rewrite up_shift_sub.
-          assert (Hlt : size body < size (tFix A body)) by (simpl; lia).
-          exact (IH body Hlt (S c0)).
-      - f_equal.
-        + apply List.map_ext_in.
-          intros p Hp.
-          pose proof (size_lt_roll_param (I:=ind) (c:=ctor) (params:=params) (recs:=recs) (p:=p) Hp) as Hlt.
-          exact (IH p Hlt c0).
-        + apply List.map_ext_in.
-          intros r Hr.
-          pose proof (size_lt_roll_rec (I:=ind) (c:=ctor) (params:=params) (recs:=recs) (r:=r) Hr) as Hlt.
-          exact (IH r Hlt c0).
-      - apply f_equal3.
-        + assert (Hlt : size scrut < size (tCase ind n scrut C brs)) by (simpl; lia).
-          exact (IH scrut Hlt c0).
-        + assert (Hlt : size C < size (tCase ind n scrut C brs)) by (simpl; lia).
-          exact (IH C Hlt c0).
-        + apply (proj1 (VectorSpec.eq_nth_iff _ _
-            (Vector.map (shift d c0) brs)
-            (Vector.map (subst (shift_sub d c0)) brs))).
-          intros p1 p2 Hp.
-          subst p2.
-          rewrite (VectorSpec.nth_map (shift d c0) brs p1 p1 eq_refl).
-          rewrite (VectorSpec.nth_map (subst (shift_sub d c0)) brs p1 p1 eq_refl).
-          pose proof (size_lt_case_branch (I:=ind) (n:=n) (scrut:=scrut) (C:=C) (brs:=brs) p1) as Hlt.
-          exact (IH (branch brs p1) Hlt c0).
-    Qed.
-
-    Lemma subst_shift0 (σ : nat -> tm) (t : tm) :
-      subst (up σ) (shift 1 0 t) = shift 1 0 (subst σ t).
-    Admitted.
-
-    Lemma up_comp_subst (σ τ : nat -> tm) :
-      forall x, up (fun y => subst σ (τ y)) x = subst (up σ) (up τ x).
-    Proof.
-      intro x.
-      destruct x as [|x]; simpl; [reflexivity|].
-      symmetry.
-      apply (subst_shift0 σ (τ x)).
-    Qed.
-
-    Lemma subst_comp (σ τ : nat -> tm) (t : tm) :
-      subst σ (subst τ t) = subst (fun x => subst σ (τ x)) t.
-    Proof.
-      revert σ τ.
-      refine (well_founded_induction wf_tm
-        (fun t => forall σ τ,
-          subst σ (subst τ t) = subst (fun x => subst σ (τ x)) t)
-        _ t).
-      intros t0 IH σ τ.
-      destruct t0 as
-        [x|i|A B|A body|fn arg|A body|ind|ind ctor params recs|ind n scrut C brs];
-        simpl; try reflexivity.
-      - f_equal.
-        + apply (IH A). simpl; lia. exact σ. exact τ.
-        + rewrite (IH B). 2: (simpl; lia). 2: exact (up σ). 2: exact (up τ).
-          apply subst_ext.
-          intro x.
-          symmetry.
-          apply up_comp_subst.
-      - f_equal.
-        + apply (IH A). simpl; lia. exact σ. exact τ.
-        + rewrite (IH body). 2: (simpl; lia). 2: exact (up σ). 2: exact (up τ).
-          apply subst_ext.
-          intro x.
-          symmetry.
-          apply up_comp_subst.
-      - f_equal.
-        + apply (IH fn). simpl; lia. exact σ. exact τ.
-        + apply (IH arg). simpl; lia. exact σ. exact τ.
-      - f_equal.
-        + apply (IH A). simpl; lia. exact σ. exact τ.
-        + rewrite (IH body). 2: (simpl; lia). 2: exact (up σ). 2: exact (up τ).
-          apply subst_ext.
-          intro x.
-          symmetry.
-          apply up_comp_subst.
-      - f_equal.
-        + apply List.map_ext_in.
-          intros p Hp.
-          apply (IH p).
-          * apply size_lt_roll_param; exact Hp.
-          * exact σ.
-          * exact τ.
-        + apply List.map_ext_in.
-          intros r Hr.
-          apply (IH r).
-          * apply size_lt_roll_rec; exact Hr.
-          * exact σ.
-          * exact τ.
-      - f_equal.
-        + apply (IH scrut). simpl; lia. exact σ. exact τ.
-        + apply (IH C). simpl; lia. exact σ. exact τ.
-        + apply Vector.map_ext.
-          intro k.
-          apply (IH (branch brs k)).
-          * apply size_lt_case_branch.
-          * exact σ.
-          * exact τ.
-    Qed.
-  End Lemmas.
+  Definition shift (d c : nat) (t : tm) : tm :=
+    rename (shift_sub d c) t.
 End Syntax.
